hs-to-coq/examples/base-thy/GHC/Base.v
@@ -8,7 +8,6 @@
  *)
 
 Require Import GHC.Base.
-Require Import GHC.BaseInstances.
 
 Require Import Coq.Logic.FunctionalExtensionality.
 
